@prefix owl:     <http://www.w3.org/2002/07/owl#> .
@prefix bim4hex:  <http://www.ibp.fraunhofer.de/ontologies/bim4hex#> .
@prefix bot:     <https://w3id.org/bot#> .
@prefix saref:   <https://w3id.org/saref#> .
@prefix xsd:     <http://www.w3.org/2001/XMLSchema#> .
@prefix rdfs:    <http://www.w3.org/2000/01/rdf-schema#> .
@prefix time4hex:  <http://www.ibp.fraunhofer.de/ontologies/time4hex#> .
@prefix rdf:     <http://www.w3.org/1999/02/22-rdf-syntax-ns#> .
@prefix hex:     <http://www.ibp.fraunhofer.de/ontologies/hex#> .
@prefix time:    <http://www.w3.org/2006/time#> .
@prefix exp:     <http://linkedearth.org/experience/ns#> .
@prefix saref4bldg:  <https://w3id.org/def/saref4bldg#> .
@prefix dc:      <http://purl.org/dc/elements/1.1/> .

dc:identifier
      a       owl:AnnotationProperty .

hex:Loud
      a       owl:Class ;
      rdfs:comment "Loudness is the subjective perception of  auditory sensation."@en ;
      rdfs:label "Loud"@en ;
      rdfs:subClassOf hex:AuditorySensation ;
      owl:disjointWith hex:Quiet .

hex:IEQFactor
      a       owl:Class ;
      rdfs:comment "A concept represents IEQ factors."@en ;
      rdfs:label "IEQFactor"@en ;
      rdfs:subClassOf
              [ a       owl:Restriction ;
                owl:onProperty hex:hasQuality ;
                owl:someValuesFrom hex:Quality
              ] .

hex:AuditorySensation
      a       owl:Class ;
      rdfs:comment "Auditory sensation is the experience of sound on ear, which can be loud or quiet."@en ;
      rdfs:label "AuditorySensation"@en ;
      rdfs:subClassOf hex:Sensation .

hex:VisualComfort
      a       owl:Class ;
      rdfs:comment "Sub-concept of IEQ factor representing visual comfort. It can be described by the combination of quality and visual sensation."@en ;
      rdfs:label "VisualComfort"@en ;
      rdfs:subClassOf hex:IEQFactor .

hex:IAQ
      a       owl:Class ;
      rdfs:comment "Sub-concept of IEQ factor representing indoor air quality. It can be described by the quality."@en ;
      rdfs:label "IAQ"@en ;
      rdfs:subClassOf hex:IEQFactor .

dc:date
      a       owl:AnnotationProperty .

hex:Quality
      a       owl:Class ;
      rdfs:comment "A concept representing the quality of relevant IE factors assessed by occupants."@en ;
      rdfs:label "Quality"@en .

hex:Cold
      a       owl:Class ;
      rdfs:comment "cold is often a subjective perception of thermal sensation."@en ;
      rdfs:label "Cold"@en ;
      rdfs:subClassOf hex:ThermalSensation ;
      owl:disjointWith hex:Warm .

hex:QuietAcousticComfort
      a       owl:Class ;
      rdfs:comment "A concepts represents acoustic comfort which has been sensed by occpuants as quiet."@en ;
      rdfs:label "QuietAcousticComfort"@en ;
      rdfs:subClassOf hex:AcousticComfort ;
      owl:equivalentClass
              [ a       owl:Class ;
                owl:intersectionOf (hex:AcousticComfort [ a       owl:Restriction ;
                            owl:onProperty hex:hasAuditorySensation ;
                            owl:someValuesFrom hex:Quiet
                          ] [ a       owl:Restriction ;
                            owl:allValuesFrom hex:Quiet ;
                            owl:onProperty hex:hasAuditorySensation
                          ])
              ] .

hex:NegativeIEQFactor
      a       owl:Class ;
      rdfs:comment "A concept represents the IEQ factors which have been assesssed as negative by occupants."@en ;
      rdfs:label "NegativeIEQFactor"@en ;
      rdfs:subClassOf hex:IEQFactor .

hex:GoodExperience
      a       owl:Class ;
      rdfs:comment "A concept represents expereiences which have all positive IEQ factors."@en ;
      rdfs:label "GoodExperience"@en ;
      rdfs:subClassOf exp:Experience ;
      owl:equivalentClass
              [ a       owl:Class ;
                owl:intersectionOf (exp:Experience [ a       owl:Restriction ;
                            owl:onProperty hex:isAbout ;
                            owl:someValuesFrom
                                    [ a       owl:Class ;
                                      owl:intersectionOf (hex:AcousticComfort hex:PositiveIEQFactor)
                                    ]
                          ] [ a       owl:Restriction ;
                            owl:onProperty hex:isAbout ;
                            owl:someValuesFrom
                                    [ a       owl:Class ;
                                      owl:intersectionOf (hex:IAQ hex:PositiveIEQFactor)
                                    ]
                          ] [ a       owl:Restriction ;
                            owl:onProperty hex:isAbout ;
                            owl:someValuesFrom
                                    [ a       owl:Class ;
                                      owl:intersectionOf (hex:PositiveIEQFactor hex:ThermalComfort)
                                    ]
                          ] [ a       owl:Restriction ;
                            owl:onProperty hex:isAbout ;
                            owl:someValuesFrom
                                    [ a       owl:Class ;
                                      owl:intersectionOf (hex:PositiveIEQFactor hex:VisualComfort)
                                    ]
                          ])
              ] .

hex:VisualSensation
      a       owl:Class ;
      rdfs:comment "A concept represents visual sensation which is the experience of light in the eye."@en ;
      rdfs:label "VisualSensation"@en ;
      rdfs:subClassOf hex:Sensation .

hex:WarmThermalComfort
      a       owl:Class ;
      rdfs:comment "A concepts represents thermal comfort which has been sensed by occpuants as warm."@en ;
      rdfs:label "WarmThermalComfort"@en ;
      rdfs:subClassOf hex:ThermalComfort ;
      owl:equivalentClass
              [ a       owl:Class ;
                owl:intersectionOf (hex:ThermalComfort [ a       owl:Restriction ;
                            owl:onProperty hex:hasThermalSensation ;
                            owl:someValuesFrom hex:Warm
                          ] [ a       owl:Restriction ;
                            owl:allValuesFrom hex:Warm ;
                            owl:onProperty hex:hasThermalSensation
                          ])
              ] .

dc:creator
      a       owl:AnnotationProperty .

dc:contributor
      a       owl:AnnotationProperty .

hex:Quiet
      a       owl:Class ;
      rdfs:comment "Quietness is the subjective perception of  auditory sensation."@en ;
      rdfs:label "Quiet"@en ;
      rdfs:subClassOf hex:AuditorySensation .

<http://www.ibp.fraunhofer.de/ontologies/hex>
      a       owl:Ontology ;
      rdfs:comment "The ontology formally represents human experiencse about IEQ factors, such as thermal comfort, visual comfort , acoustic comfort and IAQ (Indoor Air Quality). It can intregate with time ontology and bim4hex."@en ;
      dc:contributor "Georg Schneider (georg.schneider@ibp.fraunhofer.de)"@en ;
      dc:creator "Haonan Qiu (haonan.qiu@th-nurenberg.de)"@en ;
      dc:date "30.11.2017"@en ;
      dc:description "OWL ontology for human experience which can be integerated with time ontology and building related ontologies."@en ;
      dc:language "en"@en ;
      dc:title "Hex Ontology"@en ;
      owl:versionIRI <http://www.ibp.fraunhofer.de/ontologies/hex_1.0> ;
      owl:versionInfo "1.0"@en .

hex:LoudAcousticComfort
      a       owl:Class ;
      rdfs:comment "A concepts represents acoustic comfort which has been sensed by occpuants as loud."@en ;
      rdfs:label "LoudAcousticComfort"@en ;
      rdfs:subClassOf hex:AcousticComfort ;
      owl:equivalentClass
              [ a       owl:Class ;
                owl:intersectionOf (hex:AcousticComfort [ a       owl:Restriction ;
                            owl:onProperty hex:hasAuditorySensation ;
                            owl:someValuesFrom hex:Loud
                          ] [ a       owl:Restriction ;
                            owl:allValuesFrom hex:Loud ;
                            owl:onProperty hex:hasAuditorySensation
                          ])
              ] .

hex:hasQuality
      a       owl:ObjectProperty ;
      rdfs:domain hex:IEQFactor ;
      rdfs:label "hasQuality"@en ;
      rdfs:range hex:Quality .

hex:Positive
      a       owl:Class ;
      rdfs:comment "A concept represents positive"@en ;
      rdfs:label "Positive"@en ;
      rdfs:subClassOf hex:Quality .

hex:withObjectSetting
      a       owl:ObjectProperty ;
      rdfs:domain exp:Experience ;
      rdfs:label "withObjectSetting"@en ;
      rdfs:range bim4hex:Setting .

[]    a       owl:AllDisjointClasses ;
      owl:members (hex:AuditorySensation hex:ThermalSensation hex:VisualSensation) .

hex:hasVisualSensation
      a       owl:FunctionalProperty , owl:ObjectProperty ;
      rdfs:domain hex:VisualComfort ;
      rdfs:label "hasVisualSensation"@en ;
      rdfs:range hex:VisualSensation .

hex:Neutral
      a       owl:Class ;
      rdfs:comment "A concept represent neutral"@en ;
      rdfs:label "Neutral"@en ;
      rdfs:subClassOf hex:Quality .

dc:title
      a       owl:AnnotationProperty .

[]    a       owl:AllDisjointClasses ;
      owl:members (hex:Negative hex:Neutral hex:Positive) .

bim4hex:Setting
      a       owl:Class ;
      rdfs:comment "Building objects settings."@en ;
      rdfs:isDefinedBy "http://www.ibp.fraunhofer.de/ontologies/bim4hex#"@en ;
      rdfs:label "Setting"@en .

hex:ThermalComfort
      a       owl:Class ;
      rdfs:comment "Sub-concept of IEQ factor representing thermal comfort. It can be described by the combination of quality and thermal sensation."@en ;
      rdfs:label "ThermalComfort"@en ;
      rdfs:subClassOf hex:IEQFactor .

hex:Sensation
      a       owl:Class ;
      rdfs:comment "A concept represents the sensation of human in terms of indoor environment."@en ;
      rdfs:label "Sensation"@en .

time:Instant
      a       owl:Class ;
      rdfs:isDefinedBy "http://www.w3.org/2006/time#"@en ;
      rdfs:label "Instant"@en .

dc:description
      a       owl:AnnotationProperty .

hex:BadExperience
      a       owl:Class ;
      rdfs:comment "A concept represents expereiences which have all negative IEQ factors."@en ;
      rdfs:label "BadExperience"@en ;
      rdfs:subClassOf exp:Experience ;
      owl:equivalentClass
              [ a       owl:Class ;
                owl:intersectionOf (exp:Experience [ a       owl:Restriction ;
                            owl:onProperty hex:isAbout ;
                            owl:someValuesFrom
                                    [ a       owl:Class ;
                                      owl:intersectionOf (hex:AcousticComfort hex:NegativeIEQFactor)
                                    ]
                          ] [ a       owl:Restriction ;
                            owl:onProperty hex:isAbout ;
                            owl:someValuesFrom
                                    [ a       owl:Class ;
                                      owl:intersectionOf (hex:IAQ hex:NegativeIEQFactor)
                                    ]
                          ] [ a       owl:Restriction ;
                            owl:onProperty hex:isAbout ;
                            owl:someValuesFrom
                                    [ a       owl:Class ;
                                      owl:intersectionOf (hex:NegativeIEQFactor hex:ThermalComfort)
                                    ]
                          ] [ a       owl:Restriction ;
                            owl:onProperty hex:isAbout ;
                            owl:someValuesFrom
                                    [ a       owl:Class ;
                                      owl:intersectionOf (hex:NegativeIEQFactor hex:VisualComfort)
                                    ]
                          ])
              ] .

hex:Warm
      a       owl:Class ;
      rdfs:comment "Warm is often a subjective perception of thermal sensation."@en ;
      rdfs:label "Warm"@en ;
      rdfs:subClassOf hex:ThermalSensation .

hex:AcousticComfort
      a       owl:Class ;
      rdfs:comment "A concept of IEQ factor representing acoustic comfort. It can be described by the combination of quality and acoustic sensation."@en ;
      rdfs:label "AcousticComfort"@en ;
      rdfs:subClassOf hex:IEQFactor ;
      owl:equivalentClass
              [ a       owl:Class ;
                owl:intersectionOf (hex:IEQFactor [ a       owl:Restriction ;
                            owl:onProperty hex:hasAuditorySensation ;
                            owl:someValuesFrom hex:AuditorySensation
                          ])
              ] .

hex:isAbout
      a       owl:ObjectProperty ;
      rdfs:domain exp:Experience ;
      rdfs:label "isAbout"@en ;
      rdfs:range hex:IEQFactor .

hex:hasAuditorySensation
      a       owl:FunctionalProperty , owl:ObjectProperty ;
      rdfs:domain hex:AcousticComfort ;
      rdfs:label "hasAuditorySensation"@en ;
      rdfs:range hex:AuditorySensation .

hex:hasThermalSensation
      a       owl:FunctionalProperty , owl:ObjectProperty ;
      rdfs:domain hex:ThermalComfort ;
      rdfs:label "hasThermalSensation"@en ;
      rdfs:range hex:ThermalSensation .

hex:NeutralIEQFactor
      a       owl:Class ;
      rdfs:comment "A concept represents the IEQ factors which have been assesssed as neutral by occupants."@en ;
      rdfs:label "NeutralIEQFactor"@en ;
      rdfs:subClassOf hex:IEQFactor .

exp:hasTime
      a       owl:ObjectProperty ;
      rdfs:label "hasTime"@en .

saref4bldg:BuildingSpace
      a       owl:Class ;
      rdfs:isDefinedBy "https://w3id.org/def/saref4bldg#"@en ;
      rdfs:label "BuildingSpace"@en .

hex:Bright
      a       owl:Class ;
      rdfs:comment "A cocept describes that people experience light as bright."@en ;
      rdfs:label "Bright"@en ;
      rdfs:subClassOf hex:VisualSensation ;
      owl:disjointWith hex:Dim .

exp:hasLocation
      a       owl:FunctionalProperty , owl:ObjectProperty ;
      rdfs:domain exp:Experience ;
      rdfs:label "hasLocation"@en ;
      rdfs:range saref4bldg:BuildingSpace .

exp:Experience
      a       owl:Class ;
      rdfs:comment "A concpet desicrbes occupants perspectives of indoor environemental quality."@en ;
      rdfs:label "Experience"@en ;
      rdfs:subClassOf
              [ a       owl:Restriction ;
                owl:maxQualifiedCardinality
                        "1"^^xsd:nonNegativeInteger ;
                owl:onClass hex:AcousticComfort ;
                owl:onProperty hex:isAbout
              ] ;
      rdfs:subClassOf
              [ a       owl:Restriction ;
                owl:maxQualifiedCardinality
                        "1"^^xsd:nonNegativeInteger ;
                owl:onClass hex:IAQ ;
                owl:onProperty hex:isAbout
              ] ;
      rdfs:subClassOf
              [ a       owl:Restriction ;
                owl:maxQualifiedCardinality
                        "1"^^xsd:nonNegativeInteger ;
                owl:onClass hex:ThermalComfort ;
                owl:onProperty hex:isAbout
              ] ;
      rdfs:subClassOf
              [ a       owl:Restriction ;
                owl:maxQualifiedCardinality
                        "1"^^xsd:nonNegativeInteger ;
                owl:onClass hex:VisualComfort ;
                owl:onProperty hex:isAbout
              ] ;
      rdfs:subClassOf
              [ a       owl:Restriction ;
                owl:onProperty hex:withObjectSetting ;
                owl:someValuesFrom bim4hex:Setting
              ] ;
      rdfs:subClassOf
              [ a       owl:Restriction ;
                owl:onProperty exp:hasLocation ;
                owl:someValuesFrom saref4bldg:BuildingSpace
              ] ;
      rdfs:subClassOf
              [ a       owl:Restriction ;
                owl:onProperty exp:hasTime ;
                owl:someValuesFrom time:Instant
              ] .

hex:DimVisualComfort
      a       owl:Class ;
      rdfs:comment "A concept represents those visual comfort which has been sensed as dim by occupants."@en ;
      rdfs:label "DimVisualComfort"@en ;
      rdfs:subClassOf hex:VisualComfort ;
      owl:equivalentClass
              [ a       owl:Class ;
                owl:intersectionOf (hex:VisualComfort [ a       owl:Restriction ;
                            owl:onProperty hex:hasVisualSensation ;
                            owl:someValuesFrom hex:Dim
                          ] [ a       owl:Restriction ;
                            owl:allValuesFrom hex:Dim ;
                            owl:onProperty hex:hasVisualSensation
                          ])
              ] .

hex:Dim
      a       owl:Class ;
      rdfs:comment "A cocept describes that people experience light as dim."@en ;
      rdfs:label "Dim"@en ;
      rdfs:subClassOf hex:VisualSensation .

hex:ThermalSensation
      a       owl:Class ;
      rdfs:comment "Thermal sensation is a concept representing  how people ’feel’ and would typically classify their thermal states using words such as warm and cold."@en ;
      rdfs:label "ThermalSensation"@en ;
      rdfs:subClassOf hex:Sensation .

dc:language
      a       owl:AnnotationProperty .

hex:NeutralExperience
      a       owl:Class ;
      rdfs:comment "A concept represents expereiences which have all neutral IEQ factors."@en ;
      rdfs:label "NeutralExperience"@en ;
      rdfs:subClassOf exp:Experience ;
      owl:equivalentClass
              [ a       owl:Class ;
                owl:intersectionOf (exp:Experience [ a       owl:Restriction ;
                            owl:onProperty hex:isAbout ;
                            owl:someValuesFrom
                                    [ a       owl:Class ;
                                      owl:intersectionOf (hex:AcousticComfort hex:NeutralIEQFactor)
                                    ]
                          ] [ a       owl:Restriction ;
                            owl:onProperty hex:isAbout ;
                            owl:someValuesFrom
                                    [ a       owl:Class ;
                                      owl:intersectionOf (hex:IAQ hex:NeutralIEQFactor)
                                    ]
                          ] [ a       owl:Restriction ;
                            owl:onProperty hex:isAbout ;
                            owl:someValuesFrom
                                    [ a       owl:Class ;
                                      owl:intersectionOf (hex:NeutralIEQFactor hex:ThermalComfort)
                                    ]
                          ] [ a       owl:Restriction ;
                            owl:onProperty hex:isAbout ;
                            owl:someValuesFrom
                                    [ a       owl:Class ;
                                      owl:intersectionOf (hex:NeutralIEQFactor hex:VisualComfort)
                                    ]
                          ])
              ] .

hex:BrightVisualComfort
      a       owl:Class ;
      rdfs:comment "A concept represents those visual comfort which has been sensed as birght by occupants."@en ;
      rdfs:label "BrightVisualComfort"@en ;
      rdfs:subClassOf hex:VisualComfort ;
      owl:equivalentClass
              [ a       owl:Class ;
                owl:intersectionOf (hex:VisualComfort [ a       owl:Restriction ;
                            owl:onProperty hex:hasVisualSensation ;
                            owl:someValuesFrom hex:Bright
                          ] [ a       owl:Restriction ;
                            owl:allValuesFrom hex:Bright ;
                            owl:onProperty hex:hasVisualSensation
                          ])
              ] .

hex:PositiveIEQFactor
      a       owl:Class ;
      rdfs:comment "A concept represents the IEQ factors which have been assesssed as positive by occupants."@en ;
      rdfs:label "PositiveIEQFactor"@en ;
      rdfs:subClassOf hex:IEQFactor .

hex:ColdThermalComfort
      a       owl:Class ;
      rdfs:comment "A concepts represents thermal comfort which has been sensed by occpuants as cold."@en ;
      rdfs:label "ColdThermalComfort"@en ;
      rdfs:subClassOf hex:ThermalComfort ;
      owl:equivalentClass
              [ a       owl:Class ;
                owl:intersectionOf (hex:ThermalComfort [ a       owl:Restriction ;
                            owl:onProperty hex:hasThermalSensation ;
                            owl:someValuesFrom hex:Cold
                          ] [ a       owl:Restriction ;
                            owl:allValuesFrom hex:Cold ;
                            owl:onProperty hex:hasThermalSensation
                          ])
              ] .

hex:Negative
      a       owl:Class ;
      rdfs:comment "A concept represents negative."@en ;
      rdfs:label "Negative"@en ;
      rdfs:subClassOf hex:Quality .
